Test missing function with let

test/afp/Skew_Heap.thy
@@ -1,9 +1,13 @@
+section "Skew Heap"
+
 theory Skew_Heap
 imports
-  "~~/src/HOL/Library/Tree_Multiset"
+  "HOL-Library.Tree_Multiset"
+  "HOL-Library.Pattern_Aliases"
+  "HOL-Data_Structures.Heaps"
 begin
 
-section "Skew Heap"
+unbundle pattern_aliases
 
 text\<open>Skew heaps~\<^cite>\<open>"SleatorT-SIAM86"\<close> are possibly the simplest functional
 priority queues that have logarithmic (albeit amortized) complexity.
@@ -11,105 +15,65 @@ priority queues that have logarithmic (albeit amortized) complexity.
 The implementation below could be generalized to separate the elements from
 their priorities.\<close>
 
-type_synonym 'a heap = "'a tree"
+subsection "Merge"
 
-fun heap :: "'a::linorder heap \<Rightarrow> bool" where
-"heap Leaf = True" |
-"heap (Node l m r) =
-  (heap l \<and> heap r \<and> (\<forall>x \<in> set_tree l \<union> set_tree r. m \<le> x))"
-
-
-subsection "Get Minimum"
-
-fun get_min :: "'a::linorder heap \<Rightarrow> 'a" where
-"get_min(Node l m r) = m"
-
-lemma get_min_in:
-  "h \<noteq> Leaf \<Longrightarrow> get_min h \<in> set_tree h"
-by(auto simp add: neq_Leaf_iff)
-
-lemma get_min_min:
-  "\<lbrakk> heap h; h \<noteq> Leaf \<rbrakk> \<Longrightarrow> \<forall>x \<in> set_tree h. get_min h \<le> x"
-by(auto simp add: neq_Leaf_iff)
-
-
-subsection "Meld"
-
-function meld :: "('a::linorder) heap \<Rightarrow> 'a heap \<Rightarrow> 'a heap" where
-"meld Leaf h = h" |
-"meld h Leaf = h" |
-"meld (Node l1 a1 r1) (Node l2 a2 r2) =
-   (if a1 \<le> a2 then Node (meld (Node l2 a2 r2) r1) a1 l1
-    else Node (meld (Node l1 a1 r1) r2) a2 l2)" 
+function merge :: "('a::linorder) tree \<Rightarrow> 'a tree \<Rightarrow> 'a tree" where
+"merge Leaf t = t" |
+"merge t2 Leaf = t2" |
+"merge (Node l1 a1 r1 =: t1) (Node l2 a2 r2 =: t2) =
+   (if a1 \<le> a2 then Node (merge t2 r1) a1 l1
+    else Node (merge t1 r2) a2 l2)" 
 by pat_completeness auto
 termination
-by (relation "measure (\<lambda>(x, y). size x + size y)") auto
+  by (relation "measure (\<lambda>(x, y). size x + size y)") auto
 
-lemma meld_code: "meld h1 h2 =
-  (case h1 of
-   Leaf \<Rightarrow> h2 |
-   Node l1 a1 r1 \<Rightarrow> (case h2 of
-     Leaf \<Rightarrow> h1 |
+lemma merge_code: "merge t1 t2 =
+  (case t1 of
+   Leaf \<Rightarrow> t2 |
+   Node l1 a1 r1 \<Rightarrow> (case t2 of
+     Leaf \<Rightarrow> t1 |
      Node l2 a2 r2 \<Rightarrow> 
        (if a1 \<le> a2
-        then Node (meld h2 r1) a1 l1
-        else Node (meld h1 r2) a2 l2)))"
+        then Node (merge t2 r1) a1 l1
+        else Node (merge t1 r2) a2 l2)))"
 by(auto split: tree.split)
 
-text\<open> An alternative version that always walks to the Leaf of both heaps: \<close>
-function meld2 :: "('a::linorder) heap \<Rightarrow> 'a heap \<Rightarrow> 'a heap" where
-"meld2 Leaf Leaf = Leaf" |
-"meld2 Leaf (Node l2 a2 r2) = Node (meld2 r2 Leaf) a2 l2" |
-"meld2 (Node l1 a1 r1) Leaf = Node (meld2 r1 Leaf) a1 l1" |
-"meld2 (Node l1 a1 r1) (Node l2 a2 r2) =
+text\<open>An alternative version that always walks to the Leaf of both heaps:\<close>
+function merge2 :: "('a::linorder) tree \<Rightarrow> 'a tree \<Rightarrow> 'a tree" where
+"merge2 Leaf Leaf = Leaf" |
+"merge2 Leaf (Node l2 a2 r2) = Node (merge2 r2 Leaf) a2 l2" |
+"merge2 (Node l1 a1 r1) Leaf = Node (merge2 r1 Leaf) a1 l1" |
+"merge2 (Node l1 a1 r1) (Node l2 a2 r2) =
    (if a1 \<le> a2
-    then Node (meld2 (Node l2 a2 r2) r1) a1 l1
-    else Node (meld2 (Node l1 a1 r1) r2) a2 l2)"
+    then Node (merge2 (Node l2 a2 r2) r1) a1 l1
+    else Node (merge2 (Node l1 a1 r1) r2) a2 l2)"
 by pat_completeness auto
 termination
 by (relation "measure (\<lambda>(x, y). size x + size y)") auto
 
-lemma size_meld[simp]: "size(meld t1 t2) = size t1 + size t2"
-by(induction t1 t2 rule: meld.induct) auto
+lemma size_merge: "size(merge t1 t2) = size t1 + size t2"
+by(induction t1 t2 rule: merge.induct) auto
 
-lemma size_meld2[simp]: "size(meld2 t1 t2) = size t1 + size t2"
-by(induction t1 t2 rule: meld2.induct) auto
+lemma size_merge2: "size(merge2 t1 t2) = size t1 + size t2"
+by(induction t1 t2 rule: merge2.induct) auto
 
-lemma mset_meld: "mset_tree (meld h1 h2) = mset_tree h1 + mset_tree h2"
-by (induction h1 h2 rule: meld.induct) (auto simp add: ac_simps)
+lemma mset_merge: "mset_tree (merge t1 t2) = mset_tree t1 + mset_tree t2"
+by (induction t1 t2 rule: merge.induct) (auto simp add: ac_simps)
 
-lemma set_meld: "set_tree (meld h1 h2) = set_tree h1 \<union> set_tree h2"
-by (metis mset_meld set_mset_tree set_mset_union)
+lemma set_merge: "set_tree (merge t1 t2) = set_tree t1 \<union> set_tree t2"
+by (metis mset_merge set_mset_tree set_mset_union)
 
-lemma heap_meld:
-  "heap h1 \<Longrightarrow> heap h2 \<Longrightarrow> heap (meld h1 h2)"
-by (induction h1 h2 rule: meld.induct)(auto simp: ball_Un set_meld)
+lemma heap_merge:
+  "\<lbrakk> heap t1;  heap t2 \<rbrakk> \<Longrightarrow> heap (merge t1 t2)"
+by (induction t1 t2 rule: merge.induct)(auto simp: ball_Un set_merge)
 
+interpretation skew_heap: Heap_Merge
+where merge = merge
+proof(standard, goal_cases)
+  case 1 thus ?case by(simp add: mset_merge)
+next
+  case 2 thus ?case by(simp add: heap_merge)
+qed
 
-subsection "Insert"
-
-definition insert :: "'a::linorder \<Rightarrow> 'a heap \<Rightarrow> 'a heap" where
-"insert a t = meld (Node Leaf a Leaf) t"
-
-hide_const (open) Skew_Heap.insert
-
-lemma heap_insert: "heap h \<Longrightarrow> heap (Skew_Heap.insert a h)"
-by (simp add: insert_def heap_meld)
-
-lemma mset_insert: "mset_tree (Skew_Heap.insert a h) = {#a#} + mset_tree h"
-by (auto simp: mset_meld insert_def)
-
-
-subsection "Delete minimum"
-
-fun del_min :: "'a::linorder heap \<Rightarrow> 'a heap" where
-"del_min Leaf = Leaf" |
-"del_min (Node l m r) = meld l r"
-
-lemma heap_del_min: "heap h \<Longrightarrow> heap (del_min h)"
-by (cases h) (auto simp: heap_meld)
-
-lemma mset_del_min: "mset_tree (del_min h) = mset_tree h - {# get_min h #}"
-by (cases h) (auto simp: mset_meld ac_simps)
 
 end
