test/T_Binomial_Heap.thy
@@ -1,0 +1,51 @@
+theory T_Binomial_Heap
+  imports "../src/TimingFunction" "HOL-Data_Structures.Binomial_Heap"
+begin
+
+declare [[time_prefix = "T'_"]]
+
+text \<open>Define timing function\<close>
+define_time_fun link
+define_time_0 rank
+define_time_fun ins_tree
+define_time_fun insert
+
+text \<open>Only true with link being assumed constant\<close>
+define_time_0 link
+define_time_fun merge
+
+define_time_0 root
+define_time_0 min
+define_time_fun get_min
+define_time_fun get_min_rest
+define_time_0 append
+define_time_fun rev
+define_time_fun del_min
+                 
+
+text \<open>Proove equality\<close>
+theorem link: "T'_link t1 t2 = T_link t1 t2"
+  using T'_link.elims by auto
+
+theorem ins_tree: "T'_ins_tree t1 t2 = T_ins_tree t1 t2"
+  sorry
+
+theorem "T'_insert a t = T_insert a t"
+  by (auto simp: ins_tree T_insert_def)
+
+theorem merge: "T'_merge t1 t2 = T_merge t1 t2"
+  by (induction rule: T_merge.induct) (auto simp: ins_tree)
+
+theorem "t \<noteq> [] \<Longrightarrow> T'_get_min t = T_get_min t"
+  by (induction rule: T_get_min.induct) auto
+
+theorem get_min_rest: "t \<noteq> [] \<Longrightarrow> T'_get_min_rest t = T_get_min_rest t"
+  by (induction rule: T_get_min_rest.induct) auto
+
+theorem rev: "T'_rev xs = T_rev xs"
+  by (induction xs) (auto simp: T_rev_def)
+
+theorem "t \<noteq> [] \<Longrightarrow> T'_del_min t = T_del_min t"
+  by (auto simp: get_min_rest rev T_del_min_def merge split: prod.split tree.split)
+
+end
