test/T_Braun_Trees.thy
@@ -7,12 +7,20 @@ declare [[time_prefix = "T'_"]]
 
 text \<open>Define timing function\<close>
 define_time_fun insert
-text \<open>del_min contains a let\<close>
-text \<open>del_left contains a let\<close>
-text \<open>sift_down contains a let through =:\<close>
+define_time_fun sift_down
+define_time_fun del_left
+define_time_fun del_min
 
 text \<open>Proove equality\<close>
 theorem "T'_insert a t = T_insert a t"
   by (induction t arbitrary: a) auto
+
+theorem sift_down: "T'_sift_down l a r = T_sift_down l a r"
+  sorry
+theorem del_left: "t \<noteq> \<langle>\<rangle> \<Longrightarrow> T'_del_left t = T_del_left t"
+  by (induction rule: T_del_left.induct) auto
+
+theorem "T'_del_min t = T_del_min t"
+  by (induction rule: T_del_min.induct) (auto simp: sift_down del_left split: prod.split)
 
 end
