test/T_Leftist_Heap.thy
@@ -6,10 +6,17 @@ declare [[time_prefix = "T'_"]]
 
 
 text \<open>Define timing function\<close>
-text \<open>merge contains lets\<close>
-text \<open>insert contains lets\<close>
-text \<open>del_min contains lets\<close>
+define_time_0 node
+define_time_fun merge
+define_time_fun insert
+define_time_fun del_min
 
 text \<open>Proove equality\<close>
+theorem merge: "T'_merge x y = T_merge x y"
+  by (induction rule: T_merge.induct) auto
+theorem "T'_insert x y = T_insert x y + 1"
+  by (auto simp: merge T_insert_def)
+theorem "T'_del_min t  = T_del_min t + 1"
+  by (cases t) (auto simp: merge)
 
 end
